theories/MetaTheory/SubjectReduction.v
@@ -38,40 +38,6 @@ assert (Hbody'' : Σ ;; Γ ⊢ body[x := arg] : b[x := arg]).
 eapply typing_app ; eauto.
 Qed.
 
-(** One-step reduction preserves typing. *)
-Lemma typing_red1 {s} Σ Γ (t u T : term s) :
-  typing_evar_map Σ ->
-  typing_context Σ Γ ->
-  Σ ;; Γ ⊢ t : T ->
-  Σ ⊢ t ~>₁ u ->
-  Σ ;; Γ ⊢ u : T.
-Proof.
-intros HΣ HΓ Ht Hred. depind Hred.
-- eapply typing_beta ; eauto.
-- eapply typing_evar_expand ; eauto.
-- admit.
-- apply typing_lam_inv in Ht. destruct Ht as (body_ty & HT & Hty & Hbody).
-  apply IHHred in Hbody ; auto.
-  + apply typing_conv_type with (TProd x ty body_ty).
-    * apply typing_lam ; auto.
-    * now symmetry.
-    *
-  + constructor ; auto.
-
-(*apply typing_lam_inv in Ht. destruct Ht as (body_ty & H1 & Hty & Hbody).
-  apply IHHred in Hty ; auto. rewrite Hred in H1.
-  apply typing_conv_type with (TProd x ty' body_ty).
-  + apply typing_lam.
-    * assumption.
-    *
-
-  apply typing_lam. apply IHHred.*)
-
-
-apply HΣ in H. depelim H.  depelim Ht. apply typing_evar_entry.
-
-Admitted.
-
 (** Evar expansion preserves typing. *)
 Lemma typing_evar_expand {s} Σ Γ ev ty def (T : term s) :
   typing_evar_map Σ ->
@@ -86,9 +52,188 @@ intros HΣ HΓ Hev Hentry. apply typing_conv_type with (wk ty).
   + intros i. depelim i.
 - apply typing_evar_inv in Hev. destruct Hev as (entry & H & HT).
   rewrite H in Hentry. depelim Hentry. cbn in HT. now symmetry.
-- eapply typing_type_ok ; eauto.
+- eapply typing_validity ; eauto.
 Qed.
 
+Reserved Notation "Σ ⊢ Γ1 '~>ctx' Γ2"
+  (at level 50, Γ1 at next level, Γ2 at next level).
+
+(** Context reduction. *)
+Inductive red1_context (Σ : evar_map) : forall {s}, context ∅ s -> context ∅ s -> Prop :=
+| red1_context_head {s} Γ x (ty ty' : term s) :
+    Σ ⊢ ty ~> ty' ->
+    Σ ⊢ CCons Γ x ty ~>ctx CCons Γ x ty'
+
+| red1_context_tail {s} Γ Γ' x (ty : term s) :
+    Σ ⊢ Γ ~>ctx Γ' ->
+    Σ ⊢ CCons Γ x ty ~>ctx CCons Γ' x ty
+
+where "Σ ⊢ Γ1 '~>ctx' Γ2" := (red1_context Σ Γ1 Γ2).
+
+Derive Signature for red1_context.
+
+(*Lemma typing_red1_var {s} Σ Γ (i : index s) :
+  typing_evar_map Σ ->
+  typing_context Σ Γ ->
+  forall Γ',
+    Σ ⊢ Γ ~>ctx Γ' ->
+    Σ ;; Γ' ⊢ TVar i : lookup_context i Γ.
+Proof.
+intros HΣ HΓ. induction HΓ ; intros Γ' Hred.
+- depelim Hred.
+- depelim Hred ; depelim i ; simp lookup_context ; simpl_subst.
+  + cbn in H1. depelim H1.
+    assert (Γ0 = Γ) as -> by admit.
+    assert (ty0 = ty) as -> by admit.
+    clear H1 H3 H3'.*)
+
+(** One-step reduction preserves typing. *)
+Lemma typing_red1_aux {s} Σ Γ (t T : term s) :
+  typing_evar_map Σ ->
+  typing_context Σ Γ ->
+  Σ ;; Γ ⊢ t : T ->
+  (forall t', Σ ⊢ t ~> t' -> Σ ;; Γ ⊢ t' : T) /\
+  (forall Γ', Σ ⊢ Γ ~>ctx Γ' -> Σ ;; Γ' ⊢ t : T).
+Proof.
+intros HΣ HΓ Ht. induction Ht ; (split ; [intros t' Hred | intros Γ' Hred]).
+- depelim Hred.
+- constructor.
+- depelim Hred.
+- subst. apply typing_conv_type with (lookup_context i Γ').
+  + now constructor.
+  + admit.
+  +
+admit.
+  (*
+  H1 : Σ ;; Γ ⊢ ty : TType
+  H2 : Σ ;; CCons Γ x ty ⊢ TVar I0 : wk ty
+  Hred : CCons Γ x ty ~> Γ'
+  IH: forall ty', Σ ⊢ ty ~> ty' -> Σ ;; Γ ⊢ ty' : TType
+
+  Case 1:
+    CCons Γ x ty ~> CCons Γ x ty' because Σ ⊢ ty ~> ty'
+    We need to show:
+      Σ ;; CCons Γ x ty' ⊢ TVar I0 : wk ty
+
+
+
+
+  *)
+
+- constructor.
+  + now apply IHHt1.
+  + apply IHHt2 ; auto ; now constructor.
+- depelim Hred.
+  + apply typing_conv_type with (TProd x ty' body_ty).
+    * constructor.
+      --now apply IHHt1.
+      --apply IHHt2 ; auto ; now constructor.
+    * now rewrite Hred.
+    * constructor ; auto. eapply typing_validity ; eauto.
+      constructor ; auto.
+  + constructor ; auto. apply IHHt2 ; auto. now constructor.
+- constructor.
+  + now apply IHHt1.
+  + apply IHHt2 ; auto ; now constructor.
+- depelim Hred.
+  + constructor.
+    * apply IHHt1 ; auto.
+    * apply IHHt2 ; auto ; now constructor.
+  + constructor ; auto. apply IHHt2 ; auto. now constructor.
+- apply typing_app with f_ty ; [now apply IHHt |].
+  clear f Ht IHHt. induction H ; econstructor ; try eassumption.
+  + apply H ; auto.
+  + apply H1 ; auto.
+- depelim Hred.
+  + eapply typing_beta ; eauto. apply typing_app with f_ty ; eauto.
+    revert H. apply All_spine_consequence. firstorder.
+  + apply typing_app with f_ty ; [now apply IHHt |].
+    revert H. apply All_spine_consequence. firstorder.
+  + apply typing_app with f_ty ; [assumption |].
+    clear f IHHt Ht. revert f_ty T H. induction H0.
+    * intros f_ty T H1. depelim H1. eapply All_spine_cons ; eauto.
+      --now destruct H0.
+      --apply H2 ; auto.
+      --
+    * intros f_ty T H. depelim H. econstructor ; eauto.
+      --now destruct H.
+      --now destruct H2.
+- now constructor.
+- depelim Hred. rewrite H in H0. depelim H0. cbn. unfold wk. eapply typing_rename.
+  + apply HΣ in H. depelim H. eassumption.
+  + intros i. depelim i.
+- apply typing_conv_type with A ; auto.
+  + now apply IHHt1.
+  + now apply IHHt2.
+- apply typing_conv_type with A ; auto. now apply IHHt1.
+Admitted.
+
+
+
+Definition conv_context {s} Σ (Γ Γ' : context ∅ s) :=
+  forall i,
+    Σ ⊢ lookup_context i Γ ≡ lookup_context i Γ' /\
+    Σ ;; Γ' ⊢ lookup_context i Γ : TType.
+
+Lemma typing_conv_context {s} Σ (Γ : context ∅ s) t T :
+  Σ ;; Γ ⊢ t : T ->
+  forall Γ',
+  conv_context Σ Γ Γ' ->
+  Σ ;; Γ' ⊢ t : T.
+Proof.
+intros H. induction H ; intros Γ' HΓ.
+- constructor.
+- subst. apply typing_conv_type with (lookup_context i Γ').
+  + now constructor.
+  + symmetry. apply HΓ.
+  + apply HΓ. Check typing_conv_type.
+- constructor ; auto. apply IHtyping2. intros i ; depelim i ; simp lookup_context ; simpl_subst.
+  + split ; [reflexivity |]. change TType with (rename (@rshift s x) TType).
+    eapply typing_rename ; eauto. apply typing_rshift.
+
+
+(** One-step reduction preserves typing. *)
+Lemma typing_red1 {s} Σ Γ (t u T : term s) :
+  typing_evar_map Σ ->
+  typing_context Σ Γ ->
+  Σ ;; Γ ⊢ t : T ->
+  Σ ⊢ t ~>₁ u ->
+  Σ ;; Γ ⊢ u : T.
+Proof.
+intros HΣ HΓ Ht Hred. depind Hred.
+- eapply typing_beta ; eauto.
+- eapply typing_evar_expand ; eauto.
+- pose proof (Ht' := Ht). apply typing_lam_inv in Ht'. destruct Ht' as (body_ty & HT & Hty & Hbody).
+  specialize (IHHred Γ TType HΣ HΓ Hty).
+  apply typing_conv_type with (TProd x ty' body_ty).
+  + constructor ; auto. admit.
+  + rewrite <-Hred. now symmetry.
+  + eapply typing_validity ; eauto.
+
+
+- pose proof (Ht' := Ht). apply typing_lam_inv in Ht'. destruct Ht' as (body_ty & HT & Hty & Hbody).
+  specialize (IHHred (CCons Γ x ty) body_ty HΣ). feed IHHred. { constructor ; auto. }
+  feed IHHred. { assumption. }
+  apply typing_conv_type with (TProd x ty body_ty).
+  + constructor ; auto.
+  + now symmetry.
+  + eapply typing_validity ; eauto.
+- admit.
+
+
+(*apply typing_lam_inv in Ht. destruct Ht as (body_ty & H1 & Hty & Hbody).
+  apply IHHred in Hty ; auto. rewrite Hred in H1.
+  apply typing_conv_type with (TProd x ty' body_ty).
+  + apply typing_lam.
+    * assumption.
+    *
+
+  apply typing_lam. apply IHHred.*)
+
+
+apply HΣ in H. depelim H.  depelim Ht. apply typing_evar_entry.
+
+Admitted.
 
 (** Changing a term to a convertible one doesn't change its type. *)
 Lemma typing_conv {s} Σ Γ (t u T : term s) :
